Pantograph/Frontend/Refactor.lean
@@ -62,7 +62,7 @@ structure Config where
 
 structure Context where
   inContext : Parser.InputContext
-  config : Config
+  config : Config := {}
 
 structure State where
   outContext : Parser.InputContext
@@ -150,7 +150,7 @@ def hasSorry (step : CompilationStep) : Bool :=
     !nodes.isEmpty
 
 /-- Scroll to the end of the file, reading all compilation units in the process  -/
-def preprocessRefactor : FrontendM (List Command) := mapCompilationSteps λ step => do
+def preprocess : FrontendM (List Command) := mapCompilationSteps λ step => do
   let constants ← step.newConstants
   let dependencies := constants.fold (init := NameSet.empty) λ acc c =>
     acc.union $ constantDependencies step.after c
@@ -174,7 +174,7 @@ def preprocessRefactor : FrontendM (List Command) := mapCompilationSteps λ step
   return unit
 
 /-- Creates `combine (combine a[0] a[1]) a[2] ...` -/
-private def mkProdElem (combine : Name := ``And.intro) : List Expr → MetaM Expr
+def mkProdElem (combine : Name := ``And.intro) : List Expr → MetaM Expr
   | .nil => return .const `Unit []
   | [a] => return a
   | x :: xs => do
@@ -214,12 +214,13 @@ def foldTheoremsFlat (head : Command) (tail : List Command) : RefactorM Format :
     let s := comment.getDocString
     if s.isEmpty then .none else s
   let headName := head.constants.toList.head!
-  let .str _ binderName := headName
-    | panic! s!"head name must be .str but it is {headName}"
+  let binderName := match headName with
+    | .str _ binderName => Name.mkSimple binderName
+    | _ => `x
   let coreOptions ← readCoreOptions
   distilSearchTarget head tail λ witness companions => do
     -- Construct the companion
-    let companion ← Meta.withLocalDeclD (Name.mkSimple binderName) witness λ binder => do
+    let companion ← Meta.withLocalDeclD binderName witness λ binder => do
       let companion ← mkProdElem ``And.intro <| companions.map (·.instantiate1 binder)
       Meta.mkLambdaFVars #[binder] companion
     let target ← Meta.mkAppOptM ``Subtype #[witness, companion]
@@ -237,6 +238,49 @@ structure DependencyTracker where
   innerConstants : NameSet := {}
 
   isNonFlat : Bool := false
+structure DependencyStructure where
+  -- Commands which depend on each other
+  component : List Command := []
+  -- Intercalating commands
+  intercalating : List Command := []
+  -- Remainder
+  tail : List Command
+  -- Structure
+  tracker : DependencyTracker
+
+def extractDependencyStructure (head : Command) (commands : List Command)
+  : RefactorM DependencyStructure := do
+  let ((series, other), tracker) := (λ (z : StateM DependencyTracker _) => z.run {}) $
+    commands.zipIdx.partitionM λ (command, _) => do
+      let tracker ← get
+      if command.dependencies.any tracker.innerConstants.contains then
+        let innerConstants := command.constants.fold
+          (init := tracker.innerConstants)
+          λ acc n => acc.insert n
+        modify ({· with innerConstants, isNonFlat := true})
+        return true
+      if command.dependencies.any head.constants.contains then
+        let innerConstants := command.constants.fold
+          (init := tracker.innerConstants)
+          λ acc n => acc.insert n
+        modify ({· with innerConstants })
+        return true
+      else
+        return false
+  if series.isEmpty then
+    return {
+      tail := commands,
+      tracker,
+    }
+  -- Find all intercalating declarations
+  let maxIdx := series.map Prod.snd |>.max?.get!
+  let (intercalating, tail) := other.partition λ (_, idx) => idx < maxIdx
+  return {
+    component := series.map Prod.fst,
+    intercalating := intercalating.map Prod.fst,
+    tail := tail.map Prod.fst,
+    tracker
+  }
 
 /-- Scroll one unit down from the top -/
 def collectNextCommand : RefactorM Unit := do
@@ -248,42 +292,20 @@ def collectNextCommand : RefactorM Unit := do
     pushNewCommand' (⟨decl.stx⟩ : Syntax.Command)
     return
 
-  -- This keeps track of two `NameSet`s. If the dependency structure is
-  -- non-flat, we cannot refactor this.
-  let ((series, commands), tracker) := (λ (z : StateM DependencyTracker _) => z.run {}) $
-    commands.zipIdx.partitionM λ (command, _) => do
-      let tracker ← get
-      if command.dependencies.any tracker.innerConstants.contains then
-        let innerConstants := command.constants.fold
-          (init := tracker.innerConstants)
-          λ acc n => acc.insert n
-        modify ({· with innerConstants, isNonFlat := true})
-        return true
-      if command.dependencies.any decl.constants.contains then
-        let innerConstants := command.constants.fold
-          (init := tracker.innerConstants)
-          λ acc n => acc.insert n
-        modify ({· with innerConstants })
-        return true
-      else
-        return false
-  if series.isEmpty then
+  let depstr ← extractDependencyStructure decl commands
+  if depstr.component.isEmpty then
     pushNewCommand' (⟨decl.stx⟩ : Syntax.Command)
     return
-  -- Find all intercalating declarations and just run them
-  let maxIdx := series.map Prod.snd |>.max?.get!
-  let (intercalating, tail) := commands.partition λ (_, idx) => idx < maxIdx
-  -- `series` should then be rolled into a single declaration
-  modify ({ · with commands := tail.map Prod.fst })
 
-  if tracker.isNonFlat then
+  if depstr.tracker.isNonFlat then
     Refactor.fail "Cannot refactor non-flat dependency structure"
+  modify ({ · with commands := depstr.tail })
 
   -- Push all intercalating commands
-  for (command, _) in intercalating do
+  for command in depstr.intercalating do
     pushNewCommand' (⟨command.stx⟩ : Syntax.Command)
 
-  let f ← foldTheoremsFlat decl (series.map Prod.fst)
+  let f ← foldTheoremsFlat decl depstr.component
   pushNewCommand f
 
 def messageHasError := "File has error!"
@@ -294,7 +316,7 @@ open Refactor in
 def runRefactor (env : Environment) (source : String) (config : Refactor.Config := {}) : IO String := do
   let filename := "<anonymous>"
   let (fContext, fState) ← createContextStateFromFile source filename env {}
-  let commands ← preprocessRefactor.run {} |>.run fContext |>.run' fState
+  let commands ← preprocess.run {} |>.run fContext |>.run' fState
   if commands.any (·.hasError) then
     throw $ IO.userError messageHasError
   let m : RefactorM Unit := do
